WIP: add more basic results on cores

ExistentialRules/Models/Cores.lean
@@ -105,6 +105,22 @@ def injective_for_domain_list (f : α -> β) (domain : List α) : Prop := ∀ a 
 @[expose]
 def surjective_for_domain_and_image_list (f : α -> β) (domain : List α) (image : List β) : Prop := ∀ b, b ∈ image -> ∃ a, a ∈ domain ∧ f a = b
 
+/-- If a mapping is injective for a domain, then the same holds for any subset of the domain. -/
+theorem injective_of_injective_from_superset (f : α -> β) (domain : Set α) :
+    f.injective_for_domain_set domain ->
+    ∀ domain', domain' ⊆ domain -> f.injective_for_domain_set domain' := by
+  intro inj dom' dom'_sub a a' a_dom a'_dom image_eq
+  exact inj a a' (dom'_sub _ a_dom) (dom'_sub _ a'_dom) image_eq
+
+/-- The composition of two injective mappings is also injective. -/
+theorem injective_compose_of_both_injective (f : α -> β) (g : β -> γ) (domain : Set α) :
+    injective_for_domain_set f domain -> injective_for_domain_set g (f.image_set domain) ->
+    injective_for_domain_set (g ∘ f) domain := by
+  intro inj_f inj_g a a' a_dom a'_dom image_eq
+  apply inj_f a a' a_dom a'_dom
+  apply inj_g _ _ (Set.mem_map_of_mem a_dom) (Set.mem_map_of_mem a'_dom)
+  exact image_eq
+
 /-- If the composition of two mappings is injective, then the first one must be injective. -/
 theorem injective_of_injective_compose (f : α -> β) (g : β -> γ) (domain : Set α) :
     injective_for_domain_set (g ∘ f) domain -> injective_for_domain_set f domain := by
@@ -122,6 +138,18 @@ theorem surjective_of_surjective_from_subset (f : α -> β) (domain : Set α) (i
   constructor
   . apply dom'_sub; exact a_mem
   . exact a_eq
+
+/-- The composition of two surjective mappings is also surjective. -/
+theorem surjective_compose_of_both_surjective
+    (f : α -> β) (g : β -> γ) (domain : Set α) (intermediate : Set β) (image : Set γ) :
+    surjective_for_domain_and_image_set f domain intermediate ->
+    surjective_for_domain_and_image_set g intermediate image ->
+    surjective_for_domain_and_image_set (g ∘ f) domain image := by
+  intro surj_f surj_g c c_mem
+  rcases surj_g c c_mem with ⟨b, b_mem, b_eq⟩
+  rcases surj_f b b_mem with ⟨a, a_mem, a_eq⟩
+  exists a
+  simp [a_mem, a_eq, b_eq]
 
 /-- If the composition of two mappings is surjective for a domain and image, then the second one must be surjective on the same image and the domain that is the image of the first function. -/
 theorem surjective_of_surjective_compose (f : α -> β) (g : β -> γ) (domain : Set α) (image : Set γ) :
@@ -339,6 +367,52 @@ theorem strong_of_compose_strong (g h : GroundTermMapping sig) (domain : Set (Gr
     constructor
     . exact e_mem_b
     . simp
+
+/-- A `GroundTermMapping` is an isomorphism from `FactSet` A to B if
+it is a homomorphism from A to B, it is strong, injective, and surjective. -/
+@[expose]
+def isIsomorphism (h : GroundTermMapping sig) (A B : FactSet sig) : Prop :=
+  h.isHomomorphism A B ∧ h.strong A.terms A B ∧ h.injective_for_domain_set A.terms ∧ h.surjective_for_domain_and_image_set A.terms B.terms
+
+-- CAUTION: This does not hold for the current isomorphism definition.
+-- We can get an inverse but it may need to map constants to nulls, which does not make it a homomorphism.
+-- Not sure if we should have a slightly different definition or if we should just drop the result.
+theorem exists_inverse_of_isomorphism {h : GroundTermMapping sig} {A B : FactSet sig} :
+    h.isIsomorphism A B -> ∃ h' : GroundTermMapping sig, h'.isIsomorphism B A ∧ ∀ t ∈ A.terms, h' (h t) = t := by
+  intro ⟨hom, strong, inj, surj⟩
+  let h' : GroundTermMapping sig := fun t =>
+    let t_in_terms := t ∈ B.terms
+    have t_in_terms_dec := Classical.propDecidable t_in_terms
+    if mem : t_in_terms
+    then Classical.choose (surj t mem)
+    else t -- It does not matter what we return here.
+  have is_inverse : ∀ t ∈ A.terms, h' (h t) = t := by
+    intro t t_mem
+    have h_t_mem : h t ∈ B.terms := by
+      apply FactSet.terms_subset_of_subset
+      . exact hom.right
+      . rw [GroundTermMapping.terms_applyFactSet]; apply Set.mem_map_of_mem; exact t_mem
+    simp only [h', h_t_mem, ↓reduceDIte]
+    have spec := Classical.choose_spec (surj _ h_t_mem)
+    apply inj
+    . exact spec.left
+    . exact t_mem
+    . exact spec.right
+  exists h'
+  constructor
+  . constructor
+    . constructor
+      . intro c
+        simp only [h']
+        split
+        case isTrue mem =>
+          have spec := Classical.choose_spec (surj _ mem)
+          -- I DO NOT THINK THAT HOLDS ACTUALLY...
+          sorry
+        . rfl
+      . sorry
+    . sorry
+  . exact is_inverse
 
 end GroundTermMapping
 
@@ -704,7 +778,7 @@ theorem every_weakCore_isomorphic_to_strongCore_of_hom_both_ways
     (sc : FactSet sig) (sc_strong : sc.isStrongCore)
     (wc : FactSet sig) (wc_weak : wc.isWeakCore)
     (h_sc_wc h_wc_sc : GroundTermMapping sig) (h_sc_wc_hom : h_sc_wc.isHomomorphism sc wc) (h_wc_sc_hom : h_wc_sc.isHomomorphism wc sc) :
-    ∃ (iso : GroundTermMapping sig), iso.isHomomorphism wc sc ∧ iso.strong wc.terms wc sc ∧ iso.injective_for_domain_set wc.terms ∧ iso.surjective_for_domain_and_image_set wc.terms sc.terms := by
+    ∃ (iso : GroundTermMapping sig), iso.isIsomorphism wc sc := by
 
   specialize wc_weak (h_sc_wc ∘ h_wc_sc) (by
     apply GroundTermMapping.isHomomorphism_compose
@@ -752,7 +826,7 @@ theorem strongCore_unique_up_to_isomorphism_with_respect_to_weak_cores
     (fs : FactSet sig)
     (sc : FactSet sig) (sub_sc : sc.homSubset fs) (sc_strong : sc.isStrongCore)
     (wc : FactSet sig) (sub_wc : wc.homSubset fs) (wc_weak : wc.isWeakCore) :
-    ∃ (iso : GroundTermMapping sig), iso.isHomomorphism wc sc ∧ iso.strong wc.terms wc sc ∧ iso.injective_for_domain_set wc.terms ∧ iso.surjective_for_domain_and_image_set wc.terms sc.terms := by
+    ∃ (iso : GroundTermMapping sig), iso.isIsomorphism wc sc := by
 
   rcases sub_sc with ⟨sub_sc, h_fs_sc, h_fs_sc_hom⟩
   rcases sub_wc with ⟨sub_wc, h_fs_wc, h_fs_wc_hom⟩
@@ -780,7 +854,7 @@ theorem every_universal_weakCore_isomorphic_to_universal_strongCore
     {kb : KnowledgeBase sig}
     (sc : FactSet sig) (sc_universal : sc.universallyModelsKb kb) (sc_strong : sc.isStrongCore)
     (wc : FactSet sig) (wc_universal : wc.universallyModelsKb kb) (wc_weak : wc.isWeakCore) :
-    ∃ (iso : GroundTermMapping sig), iso.isHomomorphism wc sc ∧ iso.strong wc.terms wc sc ∧ iso.injective_for_domain_set wc.terms ∧ iso.surjective_for_domain_and_image_set wc.terms sc.terms := by
+    ∃ (iso : GroundTermMapping sig), iso.isIsomorphism wc sc := by
 
   rcases sc_universal.right wc wc_universal.left with ⟨h_sc_wc, h_sc_wc_hom⟩
   rcases wc_universal.right sc sc_universal.left with ⟨h_wc_sc, h_wc_sc_hom⟩
@@ -970,6 +1044,25 @@ theorem strong_core_of_universal_model_is_universal_model
       . apply TermMapping.apply_generalized_atom_set_subset_of_subset
         exact sc_sub.left
       . exact h_hom.right
+
+-- CAUTION:
+-- Not sure if this even holds. Consider F = {A(n1), A(n2)} and G = {A(c), A(d)}. There is an isomorphism from F to G but G is a weak core while F is not.
+-- (n1,n2 are nulls and c,d are constants.
+theorem weak_core_of_isomorphic_to_weak_core {fs wc : FactSet sig} (wc_core : wc.isWeakCore) :
+    (∃ iso : GroundTermMapping sig, iso.isIsomorphism fs wc) -> fs.isWeakCore := by
+  intro ⟨g, iso⟩ h endo
+  sorry
+
+theorem strong_core_of_isomorphic_to_strong_core {fs sc : FactSet sig} (sc_core : sc.isStrongCore) :
+    (∃ iso : GroundTermMapping sig, iso.isIsomorphism fs sc) -> fs.isStrongCore := by
+  intro ⟨g, iso⟩ h endo
+  have sc_weak : sc.isWeakCore := by intro h endo; exact ⟨(sc_core h endo).left, (sc_core h endo).right.left⟩
+  have weak := weak_core_of_isomorphic_to_weak_core sc_weak ⟨g, iso⟩ h endo
+  constructor
+  . exact weak.left
+  constructor
+  . exact weak.right
+  . sorry
 
 end FactSet
 
